models/simlin/RGISimulationSet.v
@@ -1,0 +1,495 @@
+Require Import FMapPositive.
+Require Import Coq.PArith.PArith.
+Require Import Coq.Program.Equality.
+Require Import Classical.
+Require Import Relation_Operators Operators_Properties.
+Require Import Coq.Classes.RelationClasses.
+
+Require Import coqrel.LogicalRelations.
+Require Import models.EffectSignatures.
+Require Import LinCCAL.
+Require Import LTS.
+Require Import Lang.
+Require Import Semantics.
+Require Import Assertion.
+Require Import TPSimulationSet.
+
+
+Module RGISimulation.
+  Import Reg.
+  Import LinCCALBase.
+  Import LTSSpec.
+  Import Semantics.
+  Import AssertionsSet.
+  Import TPSimulation.
+
+  Section Simulations.
+    Context {E : Op.t}.
+    Context {F : Op.t}.
+    Context {VE : @LTS E}.
+    Context {VF : @LTS F}.
+    Context (M : ModuleImpl E F).
+
+    CoInductive RGISimulation (R G : @RGRelation _ _ VE VF) (I : @Assertion _ _ VE VF) t (σ : State VE) c (Δ : AbstractConfig VF) : Prop :=
+    | RGISim_Error ρ π
+      (Hinvariant : I (σ, Δ))
+      (Hposs : Δ ρ π)
+      (Herror : poss_steps (PossOk ρ π) (PossError))
+    | RGISim_Continue
+      (rgisim_invstep : forall f c'
+        (Hstep : invstep M t f c c'),
+          (Ginv t f ⊆ G)%RGRelation /\
+          (forall ρ π, Δ ρ π -> TMap.find t π = None) /\
+          RGISimulation R G I t σ c' (ac_inv Δ t f))
+      (rgisim_retstep : forall f ret c'
+        (Hstep : retstep t f ret c c'),
+          (Gret t f ret ⊆ G)%RGRelation /\
+          (forall ρ π, Δ ρ π -> TMap.find t π = Some (ls_linr f ret)) /\
+          RGISimulation R G I t σ c' (ac_res Δ t))
+      (rgisim_ustep : forall ev σ' c'
+        (Hstep : ustep (Build_ThreadEvent t ev) σ c σ' c'),
+          exists Δ', (Δ' ⊆ ac_steps Δ)%AbstractConfig /\
+            G (σ, Δ) (σ', Δ') /\
+            RGISimulation R G I t σ' c' Δ')
+      (rgisim_linstep :
+          exists Δ', (Δ' ⊆ ac_steps Δ)%AbstractConfig /\
+          G (σ, Δ) (σ, Δ') /\
+          RGISimulation R G I t σ c Δ')
+      (rgisim_taustep : forall c' (Hstep : taustep t c c'),
+        RGISimulation R G I t σ c' Δ)
+
+      (rgisim_invariant : I (σ, Δ))
+      (rgisim_stable : forall σ' Δ'
+        (Hrely : R (σ, Δ) (σ', Δ'))
+        (Hinvariant : I (σ', Δ')),
+          RGISimulation R G I t σ' c Δ')
+
+      (rgisim_noerror : forall ev, ~ uerror (Build_ThreadEvent t ev) σ c)
+      (tpsim_nonemp : exists ρ π, Δ ρ π)
+    .
+
+    Variant RGISimulation_invariant (R G : RGRelation) (I : Assertion) t (X : State VE -> ThreadPoolState -> AbstractConfig VF -> Prop) σ c (Δ : AbstractConfig VF): Prop := 
+    | RGISim_Inv_Error ρ π
+      (Hinvariant : I (σ, Δ))
+      (Hposs : Δ ρ π)
+      (Herror : poss_steps (PossOk ρ π) (PossError))
+    | RGISim_Inv_Continue
+      (rgisim_invstep : forall f c'
+        (Hstep : invstep M t f c c'),
+          (Ginv t f ⊆ G)%RGRelation /\
+          (forall ρ π, Δ ρ π -> TMap.find t π = None) /\
+          X σ c' (ac_inv Δ t f))
+      (rgisim_retstep : forall f ret c'
+        (Hstep : retstep t f ret c c'),
+          (Gret t f ret ⊆ G)%RGRelation /\
+          (forall ρ π, Δ ρ π -> TMap.find t π = Some (ls_linr f ret)) /\
+          X σ c' (ac_res Δ t))
+      (rgisim_ustep : forall ev σ' c'
+        (Hstep : ustep (Build_ThreadEvent t ev) σ c σ' c'),
+          exists Δ', (Δ' ⊆ ac_steps Δ)%AbstractConfig /\
+            G (σ, Δ) (σ', Δ') /\
+            X σ' c' Δ')
+      (rgisim_linstep :
+          exists Δ', (Δ' ⊆ ac_steps Δ)%AbstractConfig /\
+          G (σ, Δ) (σ, Δ') /\
+          X σ c Δ')
+      (rgisim_taustep : forall c' (Hstep : taustep t c c'),
+        X σ c' Δ)
+
+      (rgisim_invariant : I (σ, Δ))
+      (rgisim_stable : forall σ' Δ'
+        (Hrely : R (σ, Δ) (σ', Δ'))
+        (Hinvariant : I (σ', Δ')),
+          X σ' c Δ')
+
+      (rgisim_noerror : forall ev, ~ uerror (Build_ThreadEvent t ev) σ c)
+      (tpsim_nonemp : exists ρ π, Δ ρ π)
+    .
+
+    Lemma RGISimulation_invariant_sound R G I t (X : State VE -> ThreadPoolState -> AbstractConfig VF -> Prop):
+      (forall σ c Δ, X σ c Δ -> RGISimulation_invariant R G I t X σ c Δ) ->
+      forall σ c Δ, X σ c Δ ->
+      RGISimulation R G I t σ c Δ.
+    Proof.
+      intros ?.
+      cofix IH; intros.
+      apply H in H0 as [? | ?];
+      [eapply RGISim_Error; eauto|].
+      apply RGISim_Continue; intros; auto.
+      - (* inv *)
+        eapply rgisim_invstep in Hstep as [? [? ?]].
+        do 2 (split; eauto).
+      - (* ret *)
+        eapply rgisim_retstep in Hstep as [? [? ?]].
+        do 2 (split; eauto).
+      - (* ustep *)
+        eapply rgisim_ustep in Hstep as [? [? [? ?]]]; eauto.
+      - (* linstep *)
+        destruct rgisim_linstep as (? & ? & ? & ?).
+        exists x.
+        do 2 (split; try tauto).
+        apply IH; tauto.
+    Qed.
+
+    Lemma rgisim_local_cont : forall R G I t σ Δ c c',
+      TMap.find t c = TMap.find t c' ->
+      RGISimulation R G I t σ c Δ ->
+      RGISimulation R G I t σ c' Δ.
+    Proof.
+      intros ? ? ? ?.
+      cofix IH.
+      intros ? ? ? ? Hfind Hsim.
+      inversion Hsim; subst;
+      [eapply RGISim_Error; eauto|].
+      apply RGISim_Continue; intros; eauto.
+      - eapply invstep_local_determ with (c2 := c) in Hstep as [? [? ?]]; eauto.
+        specialize (rgisim_invstep _ _ H) as [? [? ?]]. do 2 (split; auto).
+        eapply IH with (c := x); auto.
+      - eapply retstep_local_determ with (c2 := c) in Hstep as [? [? ?]]; eauto.
+        specialize (rgisim_retstep _ _ _ H) as [? [? ?]].
+        do 2 (split; auto). eapply IH with (c := x); auto.
+      - eapply ustep_local_determ with (c2 := c) in Hstep as [? [? ?]]; eauto.
+        specialize (rgisim_ustep _ _ _ H) as (? & ? & ? & ?).
+        exists x0.
+        do 2 (split; auto).
+        eapply IH with (c := x); auto.
+      - destruct rgisim_linstep as (? & ? & ? & ?).
+        exists x.
+        do 2 (split; auto).
+        eapply IH with (c := c); auto.
+      - eapply taustep_local_determ with (c2 := c) in Hstep as [? [? ?]]; [|eauto].
+        specialize (rgisim_taustep _ H).
+        eapply IH with (c := x); auto.
+      - unfold not in *.
+        intros. eapply uerror_local_determ in H; eauto.
+    Qed.
+    
+    Lemma rgisim_parapllel_composition :
+      forall (R G : tid -> RGRelation) (I : Assertion)
+        (HRG : forall t1 t2, t1 <> t2 -> (G t1 ⊆ R t2)%RGRelation),
+      forall (σ : State VE) c Δ
+        (Hnonemp : exists ρ π, Δ ρ π)
+        (Htlsim : forall t, RGISimulation (R t) (G t) I t σ c Δ),
+        TPSimulation M σ c Δ.
+    Proof.
+      intros ? ? ? ?.
+      cofix IH.
+      intros.
+      assert ((exists ρ0 π0, Δ0 ρ0 π0 /\ poss_steps (ρ0, π0) PossError) \/ ~(exists ρ0 π0, Δ0 ρ0 π0 /\ poss_steps (ρ0, π0) PossError)) as [[? [? [? ?]]] | ?] by apply classic; [eapply TPSim_Error; eauto |].
+      assert (forall ρ0 π0, Δ0 ρ0 π0 -> poss_steps (ρ0, π0) PossError -> False) as Hpnoerror; [intros; eauto|clear H].
+      apply TPSim_Continue; intros; eauto.
+      - (* inv *)
+        eapply IH; intros.
+        {
+          destruct Hnonemp as [? [? ?]].
+          do 2 eexists. econstructor. eauto.
+        }
+        pose proof (Htlsim t0) as [? | ?]; [exfalso; eapply Hpnoerror; eauto|].
+        pose proof (Htlsim t1) as [? | ?]; [exfalso; eapply Hpnoerror; eauto|].
+        destruct (Pos.eq_dec t0 t1); subst;
+        specialize (rgisim_invstep _ _ Hstep) as (? & ? & ?); auto.
+        eapply rgisim_local_cont with (c := c); auto.
+        eapply invstep_local_cont; eauto.
+        apply rgisim_stable0; [|inversion H1; auto].
+        apply (HRG _ _ n), H.
+        unfold Ginv, LiftRelation_Δ.
+        do 2 (split; eauto). reflexivity.
+      - (* ret *)
+        pose proof (Htlsim t0) as [? | ?]; [exfalso; eapply Hpnoerror; eauto|].
+        specialize (rgisim_retstep _ _ _ Hstep) as [? [? ?]].
+        split; auto.
+        eapply IH; intros.
+        {
+          destruct Hnonemp as [? [? ?]].
+          do 2 eexists. econstructor. eauto.
+        }
+        pose proof (Htlsim t1) as [? | ?]; [exfalso; eapply Hpnoerror; eauto|].
+        destruct (Pos.eq_dec t0 t1); subst; auto.
+        eapply rgisim_local_cont with (c := c); auto.
+        eapply retstep_local_cont; eauto.
+        apply rgisim_stable0; [|inversion H1; auto].
+        apply (HRG _ _ n), H.
+        unfold Gret, LiftRelation_Δ.
+        do 2 (split; eauto). reflexivity.
+      - (* ustep *)
+        destruct ev as [t ev].
+        pose proof (Htlsim t) as [? | ?]; [exfalso; eapply Hpnoerror; eauto|].
+        specialize (rgisim_ustep _ _ _ Hstep) as (Δ' & ? & ? & ?).
+        exists Δ'. split; auto.
+        eapply IH; intros.
+        {
+          destruct Hnonemp as [? [? ?]].
+          inversion H1; eauto.
+        }
+        specialize (Htlsim t0) as [? | ?]; [exfalso; eapply Hpnoerror; eauto|].
+        destruct (Pos.eq_dec t t0); subst; auto.
+        eapply rgisim_local_cont with (c := c); eauto.
+        eapply ustep_local_cont; eauto.
+        apply rgisim_stable0; [|inversion H1; auto].
+        eapply HRG; eauto.
+      - exists Δ0. split; auto.
+        apply TPSimulation.ac_steps_refl.
+      - (* tau *)
+        pose proof (Htlsim t0) as [? | ?]; [exfalso; eapply Hpnoerror; eauto|].
+        specialize (rgisim_taustep _ Hstep).
+        eapply IH; eauto; intros.
+        destruct (Pos.eq_dec t1 t0); subst; auto.
+        eapply rgisim_local_cont with (c := c); eauto.
+        eapply taustep_local_cont; eauto.
+      - (* no error *)
+        destruct ev as [t ev].
+        pose proof (Htlsim t) as [? | ?]; [exfalso; eapply Hpnoerror; eauto|].
+        auto.
+    Qed.
+
+    CoInductive MethodSimulation (R G : @RGRelation _ _ VE VF) (I : Assertion) t (f : Sig.op F) (σ : State VE) p b (Δ : AbstractConfig VF) : Prop := 
+    | MSim_Error ρ π
+      (Hinvariant : I (σ, Δ))
+      (Hposs : Δ ρ π)
+      (Herror : poss_steps (PossOk ρ π) (PossError))
+    | MSim_Continue
+      (msim_ustep : forall ev σ' p' b'
+        (Hstep : ts_step f (Build_ThreadEvent t ev) σ (Build_ThreadState f p b) σ' (Build_ThreadState f p' b')),
+          exists Δ', (Δ' ⊆ ac_steps Δ)%AbstractConfig /\
+            G (σ, Δ) (σ', Δ') /\
+            MethodSimulation R G I t f σ' p' b' Δ')
+      (msim_retstep : forall ret
+          (Hretv : p = Lang.Ret ret /\ b = None),
+          (Gret t f ret ⊆ G)%RGRelation /\
+          (I (σ, ac_res Δ t)) /\
+          (forall ρ π, Δ ρ π -> TMap.find t π = Some (ls_linr f ret)))
+      (msim_linstep :
+          exists Δ', (Δ' ⊆ ac_steps Δ)%AbstractConfig /\
+          G (σ, Δ) (σ, Δ') /\
+          MethodSimulation R G I t f σ p b Δ')
+      (msim_taustep : forall p' b'
+          (Hstep : ts_taustep (Build_ThreadState f p b) (Build_ThreadState f p' b')),
+          MethodSimulation R G I t f σ p' b' Δ)
+
+      (msim_invariant : I (σ, Δ))
+      (msim_stable : forall σ' Δ'
+        (Hrely : R (σ, Δ) (σ', Δ'))
+        (Hinvariant : I (σ', Δ')),
+          MethodSimulation R G I t f σ' p b Δ')
+      
+      (msim_noerror :
+        forall ev, ~ ts_error f (Build_ThreadEvent t ev) σ (Build_ThreadState f p b))
+      (msim_nonemp : exists ρ π, Δ ρ π)
+    .
+
+    Variant MethodSimulation_invariant (R G : RGRelation) (I : Assertion) t (f : Sig.op F) (X : State VE -> Lang.Prog E (Sig.ar f) -> option (Sig.op E) -> AbstractConfig VF -> Prop) σ p b Δ : Prop := 
+    | MSim_Inv_Error ρ π
+      (Hinvariant : I (σ, Δ))
+      (Hposs : Δ ρ π)
+      (Herror : poss_steps (PossOk ρ π) (PossError))
+    | MSim_Inv_Continue
+      (msim_ustep : forall ev σ' p' b'
+        (Hstep : ts_step f (Build_ThreadEvent t ev) σ (Build_ThreadState f p b) σ' (Build_ThreadState f p' b')),
+          exists Δ', (Δ' ⊆ ac_steps Δ)%AbstractConfig /\
+            G (σ, Δ) (σ', Δ') /\
+            X σ' p' b' Δ')
+      (msim_retstep : forall ret
+          (Hretv : p = Lang.Ret ret /\ b = None),
+          (Gret t f ret ⊆ G)%RGRelation /\
+          (I (σ, ac_res Δ t)) /\
+          (forall ρ π, Δ ρ π -> TMap.find t π = Some (ls_linr f ret)))
+      (msim_linstep :
+          exists Δ', (Δ' ⊆ ac_steps Δ)%AbstractConfig /\
+          G (σ, Δ) (σ, Δ') /\
+          X σ p b Δ')
+      (msim_taustep : forall p' b'
+          (Hstep : ts_taustep (Build_ThreadState f p b) (Build_ThreadState f p' b')),
+          X σ p' b' Δ)
+
+      (msim_invariant : I (σ, Δ))
+      (msim_stable : forall σ' Δ'
+        (Hrely : R (σ, Δ) (σ', Δ'))
+        (Hinvariant : I (σ', Δ')),
+          X σ' p b Δ')
+      
+      (msim_noerror :
+        forall ev, ~ ts_error f (Build_ThreadEvent t ev) σ (Build_ThreadState f p b))
+      (msim_nonemp : exists ρ π, Δ ρ π)
+    .
+
+    Lemma MethodSimulation_invariant_sound : forall R G I t f (X : State VE ->
+  Lang.Prog E (Sig.ar f) -> option (Sig.op E) -> AbstractConfig VF -> Prop),
+      (forall σ p b Δ, X σ p b Δ -> MethodSimulation_invariant R G I t f X σ p b Δ) ->
+      forall σ p b Δ, X σ p b Δ ->
+      MethodSimulation R G I t f σ p b Δ.
+    Proof.
+      intros ? ? ? ? ? ? ?.
+      cofix IH; intros.
+      apply H in H0 as [? | ?];
+      [eapply MSim_Error; eauto|].
+      apply MSim_Continue; intros; auto.
+      - (* ustep *)
+        apply msim_ustep in Hstep as (? & ? & ? & ?).
+        exists x. do 2 (split; auto).
+      - (* linstep *)
+        destruct msim_linstep as (? & ? & ? & ?).
+        exists x. do 2 (split; auto).
+    Qed.
+
+    Record ValidRGI (R G : @RGRelation _ _ VE VF) (I : @Assertion _ _ VE VF) t : Prop := {
+      (* HGinv : forall f, (Ginv t f ⊆ G)%RGRelation; *)
+      (* HGI : forall f, (⊨ Ginv t f ⊚ I ==>> I)%Assertion; *)
+      HRinv : forall s s', R s s' -> I s' ->
+        (forall ρ π, Δ s ρ π -> TMap.find t π = None)
+        <-> (forall ρ' π', Δ s' ρ' π' -> TMap.find t π' = None);
+
+      HInonemp : forall s, I s -> exists ρ π, Δ s ρ π;
+
+      HIpconsist: forall s ρ π, I s -> Δ s ρ π -> TMap.find t π = None ->
+                    forall ρ π, Δ s ρ π -> TMap.find t π = None
+    }.
+
+    Lemma msim_sequential_composition :
+      forall (R G : RGRelation) (I : Assertion) t
+      (Hrgi : ValidRGI R G I t)
+      (Hmsim : forall f σ Δ,
+        (Ginv t f ⊚ I)%Assertion (σ, Δ) ->
+        (forall ρ π, Δ ρ π -> TMap.find t π = Some (ls_inv f)) ->
+        MethodSimulation R G I t f σ (M f) None Δ)
+      σ ρ
+      (Hinvariant : I (σ, ac_init ρ))
+      (HGinv : forall f, (Ginv t f ⊆ G)%RGRelation)
+      (HGid : forall s, G s s),
+      RGISimulation R G I t σ (@TMap.empty _) (ac_init ρ).
+    Proof.
+      remember (TMap.empty ThreadState) as c0.
+      intros ? ? ? ? ? ? ? ?.
+      assert (TMap.find t0 c0 = None) as Hfindc;
+      [ subst; rewrite PositiveMap.gempty; auto | clear Heqc0].
+      remember (ac_init ρ) as Δ0.
+      assert (exists ρ π, Δ0 ρ π) as Hnonemp;
+      [ subst; eexists; econstructor; econstructor |].
+      assert (forall ρ0 π0, Δ0 ρ0 π0 -> TMap.find t0 π0 = None) as Hfindπ;
+      [ subst; inversion 1; subst; rewrite PositiveMap.gempty; auto | clear HeqΔ0].
+      intros ? ? ?.
+
+      apply RGISimulation_invariant_sound with (X:=fun σ c (Δ : AbstractConfig VF) =>
+        (exists ρ π, Δ ρ π) /\
+        ((
+        (forall ρ π, Δ ρ π -> TMap.find t0 π = None) /\
+        TMap.find t0 c = None /\
+        I (σ, Δ))
+        \/ 
+        (exists ts, TMap.find t0 c = Some ts /\
+        MethodSimulation R G I t0 (ts_op ts) σ (ts_prog ts) (ts_pend ts) Δ))
+      ); try tauto.
+      clear - Hrgi Hmsim HGinv HGid.
+      intros.
+      destruct H as [Hnonemp [[Hfindπ [Hfindc HI]] | [ts [Hfindc Hmsim']]]].
+      (* invstep *)
+      {
+        assert ((exists ρ0 π0, Δ0 ρ0 π0 /\ poss_steps (ρ0, π0) PossError) \/ ~(exists ρ0 π0, Δ0 ρ0 π0 /\ poss_steps (ρ0, π0) PossError)) as [[? [? [? ?]]] | ?] by apply classic; [eapply RGISim_Inv_Error; eauto |].
+        assert (forall ρ0 π0, Δ0 ρ0 π0 -> poss_steps (ρ0, π0) PossError -> False) as Hpnoerror; [intros; eauto|clear H].
+        apply RGISim_Inv_Continue; intros; auto;
+        try (inversion Hstep; subst; simpl in *; congruence).
+        - inversion Hstep; subst. clear Hfind.
+          do 2 (split; auto).
+          split; [ destruct Hnonemp as [? [? ?]]; do 2 eexists; econstructor; eauto |].
+          right.
+          exists {| ts_op := f; ts_prog := M f; ts_pend := None |}.
+          rewrite PositiveMap.gss.
+          split; auto.
+          simpl.
+          eapply Hmsim.
+          * exists (σ0, Δ0).
+            split; auto.
+            unfold Ginv, LiftRelation_Δ. simpl.
+            do 2 (split; auto). reflexivity.
+          * inversion 1; subst. rewrite PositiveMap.gss. auto.
+        - exists Δ0. split; [apply TPSimulation.ac_steps_refl|].
+          split; eauto.
+        - destruct Hrgi.
+          split; [ eapply HInonemp0 in Hinvariant; eauto |].
+          left.
+          split; try tauto.
+          apply HRinv0 in Hrely; auto.
+          simpl in Hrely. apply Hrely; auto.
+        - unfold not; intros.
+          inversion H; subst; simpl in *; try congruence.
+      }
+      (* other steps *)
+      {
+        clear Hmsim; rename Hmsim' into Hmsim.
+
+        assert (I (σ0, Δ0)); [inversion Hmsim; auto|].
+        assert ((exists ρ0 π0, Δ0 ρ0 π0 /\ poss_steps (ρ0, π0) PossError) \/ ~(exists ρ0 π0, Δ0 ρ0 π0 /\ poss_steps (ρ0, π0) PossError)) as [[? [? [? ?]]] | ?] by apply classic; [eapply RGISim_Inv_Error; eauto |].
+        assert (forall ρ0 π0, Δ0 ρ0 π0 -> poss_steps (ρ0, π0) PossError -> False) as Hpnoerror; [intros; eauto|].
+        clear H H0.
+        
+        apply RGISim_Inv_Continue; intros; auto;
+        try (inversion Hstep; subst; simpl in *; congruence).
+        - (* ret *)
+          inversion Hstep; subst.
+          rewrite Hfindc in Hfind.
+          inversion Hfind; subst; clear Hfind.
+          simpl in *.
+
+          inversion Hmsim; [exfalso; eapply Hpnoerror; eauto|].
+          specialize (msim_retstep _ (conj eq_refl eq_refl)) as [? [? ?]].
+          do 2 (split; auto).
+          split; [| left; do 2 try split; auto].
+          + destruct msim_nonemp as [? [? ?]].
+            do 2 eexists; econstructor; eauto.
+          + inversion 1; subst. rewrite PositiveMap.grs. auto.
+          + rewrite PositiveMap.grs. auto.
+        - (* ustep *)
+          inversion Hstep; subst. simpl in *.
+          rewrite Hfindc in Hfind. inversion Hfind; subst.
+          clear Hfind.
+          inversion Hmsim; [exfalso; eapply Hpnoerror; eauto|].
+          destruct ts1 as [f' p b].
+          pose proof ts_step_inversion _ _ _ _ _ _ _ _ Hstep0 as [? [p' [b' ?]]]; subst.
+          simpl in *.
+          specialize (msim_ustep _ _ _ _ Hstep0) as [Δ' [? [? ?]]].
+          exists Δ'.
+          do 2 (split; auto).
+          split; [inversion H1; eauto|].
+          right.
+          exists {| ts_op := f'; ts_prog := p'; ts_pend := b' |}.
+          simpl.
+          split; auto.
+          rewrite PositiveMap.gss. auto.
+        - (* linstep *)
+          exists Δ0. split; [apply TPSimulation.ac_steps_refl |].
+          split; eauto.
+        - (* tau *)          
+          inversion Hstep; subst.
+          rewrite Hfindc in Hfind. inversion Hfind; subst.
+          inversion Hstep0; subst; simpl in *.
+          inversion Hmsim; [exfalso; eapply Hpnoerror; eauto|].
+          split; eauto.
+          apply msim_taustep in Hstep0. 
+          right.
+          exists {| ts_op := f; ts_prog := p; ts_pend := b |}.
+          split; auto.
+          rewrite PositiveMap.gss. auto.
+        - (* invariant *)
+          inversion Hmsim; auto.
+        - (* rely *)
+          split.
+          + destruct Hrgi.
+            apply HInonemp0 in Hinvariant; auto.
+          + right.
+            exists ts.
+            split; auto.
+            inversion Hmsim; [exfalso; eapply Hpnoerror; eauto|].
+            auto.
+        - (* noerror *)
+          intros ?.
+          inversion H; subst. simpl in *.
+          inversion Herror; subst. simpl in *.
+          rewrite Hfindc in Hfind.
+          inversion Hfind; subst. simpl in *.
+          inversion Hmsim; [exfalso; eapply Hpnoerror; eauto|].
+          eapply msim_noerror; eauto.
+      }
+    Qed.
+
+  End Simulations.
+
+End RGISimulation.
